Makefile
@@ -8,9 +8,12 @@ frap:
 coq: Makefile.coq frap
 	$(MAKE) -f Makefile.coq
 
+pingpong: coq
+	$(MAKE) -f Makefile.coq protocols/EncPingProtocol.vo
+
 Makefile.coq: Makefile _CoqProject
 	coq_makefile -f _CoqProject -o Makefile.coq
 
-clean:: Makefile.coq
+clean: Makefile.coq
 	$(MAKE) -f Makefile.coq clean
 	rm -f Makefile.coq
